lakefile.lean
@@ -30,7 +30,7 @@ def mcelieceFiles : Array FilePath :=
   let nist : FilePath := "nist"
   #[ nist / "rng.c",
      "benes.c", "bm.c", "controlbits.c", "decrypt.c", "encrypt.c", "gf.c",
-     "operations.c", "pk_gen.c", "root.c", "sk_gen.c", "synd.c", "transpose.c", "util.c"
+     "pk_gen.c", "root.c", "sk_gen.c", "synd.c", "transpose.c", "util.c"
     ]
 
 def mcelieceTarget (pkgDir : FilePath) (srcPath : FilePath) : FileTarget :=
