lib/Crypto.lean
@@ -5,6 +5,9 @@ import Crypto.UInt8
 def ByteVec.toBuffer {n:Nat} : ByteVec n → ByteBuffer
 | ⟨a,_⟩ => ⟨a⟩ 
 
+instance : Coe (ByteVec n) ByteBuffer where
+  coe := ByteVec.toBuffer
+
 theorem add_le_implies_le_rhs {j k : Nat} : ∀(i : Nat), (h : i + j ≤ k) → j ≤ k
 | Nat.succ i, h => add_le_implies_le_rhs i (Nat.le_of_succ_le (Nat.succ_add i j ▸ h))
 | 0, h => Nat.zero_add j ▸ h
@@ -30,20 +33,31 @@ def initKeypairSeedPrefix : ByteVec 1 := #v[64]
 
 def initKeypairSeed (v:ByteVec 32) : ByteVec 33 := initKeypairSeedPrefix ++ v
 
+@[extern "lean_crypto_hash_32b"]
+constant cryptoHash32b : ByteBuffer → ByteVec 32
+
 namespace Mceliece348864Ref
 def name : String := "mceliece348864"
 def publicKeyBytes : Nat := 261120
 def secretKeyBytes : Nat := 6492
 
 def plaintextBytes : Nat := 32
+
+@[reducible]
 def ciphertextBytes : Nat := 128 
 
 def N := 3488
 
+@[reducible]
 def gfbits : Nat := 12
+
+@[reducible]
 def sys_t : Nat := 64
+
+@[reducible]
 def pk_nrows : Nat := sys_t * gfbits
 
+@[reducible]
 def synd_bytes : Nat := ((pk_nrows + 7)/8)
 
 def PublicKey := ByteVec Mceliece348864Ref.publicKeyBytes
@@ -53,17 +67,16 @@ def SecretKey := ByteVec Mceliece348864Ref.secretKeyBytes
   deriving ToString
 
 def Plaintext := ByteVec Mceliece348864Ref.plaintextBytes
-  deriving DecidableEq, ToString
+  deriving DecidableEq, Inhabited, ToString
 
+@[reducible]
 def Ciphertext := ByteVec Mceliece348864Ref.ciphertextBytes
   deriving ToString
 
-end Mceliece348864Ref
-
 structure KeyPair where
-  pk : Mceliece348864Ref.PublicKey
-  sk : Mceliece348864Ref.SecretKey
-  
+  pk : PublicKey
+  sk : SecretKey
+
 @[extern "lean_try_crypto_kem_keypair"]
 constant tryCryptoKemKeypair (seed: ByteVec 33) : Option KeyPair × ByteVec 33
 
@@ -80,21 +93,41 @@ def mkCryptoKemKeypair (iseed : ByteVec 48) (attempts: optParam Nat 10) : IO Key
   | some p => p
 
 structure EncryptionResult where
-  ss : Mceliece348864Ref.Plaintext
-  ct : Mceliece348864Ref.Ciphertext
+  ss : Plaintext
+  ct : Ciphertext
 
 @[extern "lean_crypto_enc"]
-constant mkCryptoEnc : @&Mceliece348864Ref.PublicKey 
-                     → IO (ByteVec Mceliece348864Ref.synd_bytes × ByteVec (Mceliece348864Ref.N / 8))
+constant mkCryptoEnc : @&PublicKey 
+                     → IO (ByteVec synd_bytes × ByteVec (N / 8))
 
-@[extern "lean_crypto_hash_32b"]
-constant cryptoHash32b : ByteBuffer → ByteVec 32
-
-def mkCryptoKemEnc (pk:Mceliece348864Ref.PublicKey) : IO EncryptionResult := do
+def mkCryptoKemEnc (pk:PublicKey) : IO EncryptionResult := do
   let (c, e) ← mkCryptoEnc pk
-  let c   := c ++ cryptoHash32b (#b[2] ++ e.toBuffer)
-  let key := cryptoHash32b $ #b[1] ++ e.toBuffer ++ c.toBuffer
+  let c   := c ++ cryptoHash32b (#b[2] ++ e)
+  let key := cryptoHash32b $ #b[1] ++ e ++ c
   pure ⟨key, c⟩
- 
-@[extern "lean_crypto_kem_dec"]
-constant cryptoKemDec (ct : @&Mceliece348864Ref.Ciphertext) (sk : @&Mceliece348864Ref.SecretKey) : IO Mceliece348864Ref.Plaintext
+
+@[extern "lean_decrypt"]
+constant decrypt (ct : @&(ByteVec synd_bytes)) (sk : @&(ByteVec (secretKeyBytes - 40))) : ByteVec (N / 8) × UInt8
+
+def irr_bytes : Nat := sys_t * 2
+
+def cond_bytes : Nat := (1 <<< (gfbits-4))*(2*gfbits - 1)
+
+def cryptoKemDec (c : @&Ciphertext) (sk : @&SecretKey) : Plaintext := Id.run $ do
+  let c_cipher := c.extract 0 synd_bytes
+  let c_hash : ByteVec 32 := c.extract synd_bytes (synd_bytes+32)
+  let (e, ret_decrypt) := decrypt c_cipher (sk.drop 40)  
+  let conf := cryptoHash32b (#b[2] ++ e)
+  let ret_confirm := ByteVec.orAll (conf ^^^ c_hash)
+  let m : UInt16 := UInt16.ofNat $ UInt8.toNat (ret_decrypt ||| ret_confirm)
+  let m := m - 1
+  let m := UInt8.ofNat $ UInt16.toNat (m >>> 8)
+
+  -- Generate preimage
+  let s := sk.extract (40 + irr_bytes + cond_bytes) (40 + irr_bytes + cond_bytes + N/8)
+  let preimageX : ByteVec (N/8) := ~~~m &&& s
+  let preimageY : ByteVec (N/8) := m &&& (e.extract 0 (N/8))
+  let preimage := preimageX ||| preimageY
+  pure $ cryptoHash32b $ #b[m &&& 1] ++ preimage ++ c
+
+end Mceliece348864Ref
