lib/Crypto/ToSubarray.lean
@@ -1,0 +1,15 @@
+syntax:max term noWs "[[" term ":" term "]]" : term
+syntax:max term noWs "[[" term ":" "]]" : term
+syntax:max term noWs "[[" ":" term "]]" : term
+
+class ToSubarray (collection : Type u) (subarray : outParam (Type u)) : Type u where
+  size : collection → Nat
+  toSubarray (as : collection) (start : Nat := 0) (stop : Nat := size as) : subarray  
+
+export ToSubarray (size)
+export ToSubarray (toSubarray)
+
+macro_rules
+  | `($a[[$start : $stop]]) => `(toSubarray $a $start $stop)
+  | `($a[[ : $stop]])       => `(toSubarray $a 0 $stop)
+  | `($a[[$start : ]])      => `(toSubarray a $start a.size)
