lib/Main.lean
@@ -1,31 +1,34 @@
 import Crypto
 
-def main : IO Unit := do
-  randombytesInit (ByteVec.sequence 48);
-  let mut seedArray : Array (ByteVec 48) := #[]
-  let fpReq ← openByFd 8;
-  for i in [0:10] do
-    let seed ← randombytes 48;
-    fpReq.putStrLn $ "count = " ++ toString i
-    fpReq.putStrLn $ "seed = " ++ toString seed
-    fpReq.putStrLn "pk ="
-    fpReq.putStrLn "sk ="
-    fpReq.putStrLn "ct ="
-    fpReq.putStrLn "ss =\n"    
-    seedArray := seedArray.push seed
-  let fpRsp ← openByFd 9;
---  let fpRsp ← IO.getStdout
-  fpRsp.putStrLn $ "# kem/" ++ Mceliece348864Ref.name ++"\n"
-  for i in [0:10], seed in seedArray do
-    let key ← mkCryptoKemKeypair seed
-    let enc ← mkCryptoKemEnc key.pk
-    let ss1 ← cryptoKemDec enc.ct key.sk
-    if enc.ss ≠ ss1 then
-      throw $ IO.userError "crypto_kem_dec returned bad 'ss' value"
-    fpRsp.putStrLn $ s!"count = {i}"
-    fpRsp.putStrLn $ s!"seed = {seed}"
-    fpRsp.putStrLn $ s!"pk = {key.pk}"
-    fpRsp.putStrLn $ s!"sk = {key.sk}"
-    fpRsp.putStrLn $ s!"ct = {enc.ct}"
-    fpRsp.putStrLn $ s!"ss = {ss1}\n"  
-  IO.println "Done"
+def main (args:List String): IO Unit := do
+  match args with
+  | [reqPath, rspPath] => do
+      randombytesInit (ByteVec.sequence 48);
+      let mut seedArray : Array (ByteVec 48) := #[]
+      let fpReq ← IO.FS.Handle.mk reqPath IO.FS.Mode.write false
+      for i in [0:10] do
+        let seed ← randombytes 48;
+        fpReq.putStrLn s!"count = {i}"
+        fpReq.putStrLn s!"seed = {seed}"
+        fpReq.putStrLn "pk ="
+        fpReq.putStrLn "sk ="
+        fpReq.putStrLn "ct ="
+        fpReq.putStrLn "ss =\n"
+        seedArray := seedArray.push seed
+      let fpRsp ← IO.FS.Handle.mk rspPath IO.FS.Mode.write false
+      fpRsp.putStrLn $ s!"# kem/{Mceliece348864Ref.name}\n"
+      for i in [0:10], seed in seedArray do
+        let key ← Mceliece348864Ref.mkCryptoKemKeypair seed
+        let enc ← Mceliece348864Ref.mkCryptoKemEnc key.pk
+        let expected := Mceliece348864Ref.cryptoKemDec enc.ct key.sk
+        if enc.ss ≠ expected then
+          throw $ IO.userError "crypto_kem_dec returned bad 'ss' value"
+        fpRsp.putStrLn $ s!"count = {i}"
+        fpRsp.putStrLn $ s!"seed = {seed}"
+        fpRsp.putStrLn $ s!"pk = {key.pk}"
+        fpRsp.putStrLn $ s!"sk = {key.sk}"
+        fpRsp.putStrLn $ s!"ct = {enc.ct}"
+        fpRsp.putStrLn $ s!"ss = {enc.ss}\n"  
+      IO.println "Done"
+  | _ => do
+    throw $ IO.userError "Expected reqPath and rspPath"
