scripts/test.sh
@@ -2,6 +2,6 @@
 set -ex
 lake build
 mkdir -p tmp
-DYLD_LIBRARY_PATH="deps/openssl-1.1.1l" ./build/bin/crypto 8> tmp/kat_kem.req 9> tmp/kat_kem.rsp
+./build/bin/crypto tmp/kat_kem.req tmp/kat_kem.rsp
 cmp --silent tests/kat_kem.req.golden tmp/kat_kem.req || echo "Req files are different"
 cmp --silent tests/kat_kem.rsp.golden tmp/kat_kem.rsp || echo "Rsp files are different"
